Splinter/AllocationsLayer/CoordinationJournal.dfy
@@ -1,0 +1,198 @@
+// Copyright 2018-2021 VMware, Inc., Microsoft Inc., Carnegie Mellon University, ETH Zurich, and University of Washington
+// SPDX-License-Identifier: BSD-2-Clause
+
+include "AllocationJournal.i.dfy"
+
+module CoordinationJournal {
+  import opened Options
+  import opened ValueMessage
+  import opened KeyType
+  import opened StampedMod
+  import opened MsgHistoryMod
+  import opened LSNMod
+
+  import GenericDisk
+  import AllocationJournal
+
+  type AU = GenericDisk.AU
+
+  datatype TransitionLabel =
+    | LoadEphemeralFromPersistentLabel()
+    | ReadForRecoveryLabel(records: MsgHistory)
+    | QueryEndLsnLabel(endLsn: LSN)
+    | PutLabel(records: MsgHistory)
+    | InternalAllocationsLabel(allocs: set<AU>, deallocs: set<AU>)
+    | QueryLsnPersistenceLabel(syncLsn: LSN)
+    | CommitStartLabel(newBoundaryLsn: LSN, maxLsn: LSN, unobserved: set<AU>)
+    | CommitCompleteLabel(requireEnd: LSN, discarded: set<AU>)
+    | CrashLabel()
+
+  type StoreImage = AllocationJournal.JournalImage
+
+  datatype Ephemeral =
+    | Unknown  // This means Nones
+    | Known(v: AllocationJournal.Variables)
+  {
+    predicate WF() {
+      Known? ==> v.WF()
+    }
+  }
+
+  datatype Variables = Variables(
+    persistent: StoreImage,
+    ephemeral: Ephemeral,
+    inFlight: Option<StoreImage>
+  )
+  {
+    predicate WF() {
+      && persistent.WF()
+      && ephemeral.WF()
+      && (inFlight.Some? ==> inFlight.value.WF())
+    }
+  }
+
+  predicate LoadEphemeralFromPersistent(v: Variables, v': Variables, lbl: TransitionLabel)
+  {
+    && v.WF()
+    && lbl.LoadEphemeralFromPersistentLabel?
+    && v.ephemeral.Unknown?
+    && v'.ephemeral.Known?
+
+    && AllocationJournal.Init(v'.ephemeral.v, v.persistent)
+    && v'.persistent == v.persistent // UNCHANGED
+    && v'.inFlight == v.inFlight // UNCHANGED
+  }
+
+  predicate ReadForRecovery(v: Variables, v': Variables, lbl: TransitionLabel)
+  {
+    && v.WF()
+    && lbl.ReadForRecoveryLabel?
+    && v.ephemeral.Known?
+    && v'.ephemeral.Known?
+  
+    && AllocationJournal.Next(v.ephemeral.v, v'.ephemeral.v, AllocationJournal.ReadForRecoveryLabel(lbl.records))
+    && v' == v  // everything UNCHANGED
+  }
+  
+  predicate QueryEndLsn(v: Variables, v': Variables, lbl: TransitionLabel)
+  {
+    && v.WF()
+    && lbl.QueryEndLsnLabel?
+    && v.ephemeral.Known?
+    && v'.ephemeral.Known?
+
+    && AllocationJournal.Next(v.ephemeral.v, v'.ephemeral.v, AllocationJournal.QueryEndLsnLabel(lbl.endLsn))
+    && v' == v
+  }
+
+  predicate Put(v: Variables, v': Variables, lbl: TransitionLabel)
+  {
+    && v.WF()
+    && lbl.PutLabel?
+    && v.ephemeral.Known?
+    && v'.ephemeral.Known?
+
+    && AllocationJournal.Next(v.ephemeral.v, v'.ephemeral.v, AllocationJournal.PutLabel(lbl.records))
+    && v'.persistent == v.persistent // UNCHANGED
+    && v'.inFlight == v.inFlight // UNCHANGED
+  }
+
+  predicate Internal(v: Variables, v': Variables, lbl: TransitionLabel)
+  {
+    && v.WF()
+    && lbl.InternalAllocationsLabel?
+    && v.ephemeral.Known?
+    && v'.ephemeral.Known?
+
+    && AllocationJournal.Next(v.ephemeral.v, v'.ephemeral.v, 
+      AllocationJournal.InternalAllocationsLabel(lbl.allocs, lbl.deallocs))
+    && v'.persistent == v.persistent // UNCHANGED
+    && v'.inFlight == v.inFlight // UNCHANGED
+  }
+
+  predicate QueryLsnPersistence(v: Variables, v': Variables, lbl: TransitionLabel)
+  {
+    && v.WF()
+    && lbl.QueryLsnPersistenceLabel?
+    && lbl.syncLsn <= v.persistent.tj.SeqEnd()
+    && v' == v
+  }
+
+  predicate CommitStart(v: Variables, v': Variables, lbl: TransitionLabel)
+  {
+    && v.WF()
+    && lbl.CommitStartLabel?
+    && v.ephemeral.Known?
+    // Can't start a commit if one is in-flight, or we'd forget to maintain the
+    // invariants for the in-flight one.
+    && v.inFlight.None?
+    && v'.ephemeral.Known?
+    && v'.inFlight.Some?
+
+    && var frozenJournal := v'.inFlight.value;
+    && AllocationJournal.Next(v.ephemeral.v, v'.ephemeral.v, 
+      AllocationJournal.FreezeForCommitLabel(frozenJournal, lbl.unobserved))
+
+    // Frozen journal stitches to frozen map
+    && frozenJournal.tj.SeqStart() == lbl.newBoundaryLsn
+
+    // Journal doesn't go backwards
+    && v.persistent.tj.SeqEnd() <= frozenJournal.tj.SeqEnd()
+
+    // There should be no way for the frozen journal to have passed the ephemeral map!
+    && frozenJournal.tj.SeqStart() <= lbl.maxLsn
+
+    && v' == v.(
+      ephemeral := v'.ephemeral,  // given by predicate above (but happens to be read-only / unchanged)
+      inFlight := Some(frozenJournal) // given by predicates above
+      )
+  }
+
+  // Observe that the persistent journal is always a prefix of the Ephemeral Journal
+  predicate CommitComplete(v: Variables, v': Variables, lbl: TransitionLabel)
+  {
+    && v.WF()
+    && lbl.CommitCompleteLabel?
+    && v.ephemeral.Known?
+    && v.inFlight.Some?
+    && v'.ephemeral.Known?
+
+    && AllocationJournal.Next(v.ephemeral.v, v'.ephemeral.v,
+        AllocationJournal.DiscardOldLabel(v.inFlight.value.tj.SeqStart(), lbl.requireEnd, lbl.discarded))
+
+    && v' == v.(
+      persistent := v.inFlight.value,
+      ephemeral := v'.ephemeral,  // given by predicate above
+      inFlight := None)
+  }
+
+  predicate Crash(v: Variables, v': Variables, lbl: TransitionLabel)
+  {
+    && v.WF()
+    && lbl.CrashLabel?
+    && v' == v.(
+      ephemeral := Unknown,
+      inFlight := None)
+  }
+
+  predicate Init(v: Variables)
+  {
+    v == Variables(AllocationJournal.EmptyJournalImage(), Unknown, None)
+  }
+
+  predicate Next(v: Variables, v': Variables, lbl: TransitionLabel)
+  {
+    match lbl {
+      case LoadEphemeralFromPersistentLabel() => LoadEphemeralFromPersistent(v, v', lbl)
+      case ReadForRecoveryLabel(_) => ReadForRecovery(v, v', lbl)
+      case QueryEndLsnLabel(_) => QueryEndLsn(v, v', lbl)
+      case PutLabel(_) => Put(v, v', lbl)
+      case InternalAllocationsLabel(_, _) => Internal(v, v', lbl)
+      case QueryLsnPersistenceLabel(_) => QueryLsnPersistence(v, v', lbl)
+      case CommitStartLabel(_, _, _) => CommitStart(v, v', lbl)
+      case CommitCompleteLabel(_, _) => CommitComplete(v, v', lbl)
+      case CrashLabel() => Crash(v, v', lbl)
+    }
+  }
+}
+
